add some verification to split

parser/split.dfy
@@ -1,31 +1,158 @@
 module Split {
+    function sumSeq(ss: seq<string>, separator: string ): string {
+        if |ss| == 0 then "" else if |ss| == 1 then ss[0] else ss[0] + separator + sumSeq(ss[1..], separator)
+    }
+
+    function partialSumSeq(ss: seq<string>, separator: string ): string {
+        if |ss| == 0 then "" else ss[0] + separator + partialSumSeq(ss[1..], separator)
+    }
+
+    function sumLength(xs: seq<string>): nat {
+        if |xs| == 0 then 0 else |xs[|xs|-1]|+sumLength(xs[..|xs|-1])
+    }
+
+    function prod(x:int,y: int): int {
+        x * y
+    }
+
+    predicate nextStartingIndex(sindex: nat, separator: string, results: seq<string>) {
+        prod((|results|), |separator|) + sumLength(results) == sindex
+    }
+
+    predicate finalIndex(s: string, separator: string, results: seq<string>) {
+        prod((|results|-1), |separator|) + sumLength(results) == |s|
+    }
+
+    lemma sumSeqPartial(ss: seq<string>,  separator: string)
+        requires |ss| >0
+        ensures sumSeq(ss, separator) == partialSumSeq(ss[..|ss|-1], separator)+ss[|ss|-1]
+    {
+        if |ss| == 1 {
+
+        }else{
+            assert |ss| > 1;
+            sumSeqPartial(ss[1..], separator);
+            assert sumSeq(ss[1..], separator) == partialSumSeq(ss[1..][..|ss[1..]|-1], separator)+ss[1..][|ss[1..]|-1];
+            assert ss[|ss|-1] == ss[1..][|ss[1..]|-1];
+            assert ss[1..][..|ss[1..]|-1] == ss[1..|ss|-1];
+
+        }
+    }
+
+    lemma partialSumSeqConcat(ss:seq<string>, xx: seq<string>, separator: string)
+        ensures partialSumSeq(ss+xx, separator) == partialSumSeq(ss, separator) + partialSumSeq(xx, separator)
+    {
+        if |ss| == 0 {
+            calc {
+                ss+xx;
+                []+xx;
+                xx;
+            }
+        }else if |xx| == 0 {
+            calc {
+                ss+[];
+                ss+[];
+                ss;
+            }
+        }else {
+            assert |ss| != 0;
+            partialSumSeqConcat(ss[1..], xx, separator);
+            calc {
+                partialSumSeq(ss+xx, separator);
+                (ss+xx)[0]+separator+partialSumSeq((ss+xx)[1..],separator);
+                {
+                    assert (ss+xx)[0] == ss[0];
+                    assert (ss+xx)[1..] == ss[1..]+xx;
+                }
+                ss[0]+separator+partialSumSeq(ss[1..]+xx,separator);
+                ss[0]+separator+partialSumSeq(ss[1..], separator)+partialSumSeq(xx,separator);
+            }
+
+        }
+    }
+
+    function splitOnLetter(s: string, index: int, results: seq<string>): seq<string> 
+        requires 0 <= index <= |s|
+        requires forall i :: 0 <= i <  index <= |results| ==> s[i..i+1] == results[i]
+        requires |results| == index
+        ensures forall i :: 0 <= i < |s| <= |splitOnLetter(s, index, results)|  ==> s[i..i+1] == splitOnLetter(s, index, results)[i]
+        ensures |splitOnLetter(s, index, results)| == |s|
+        decreases |s|-index
+    {
+        if index < |s| then
+            assert index <= index +1;
+            var nextResult:= results+[s[index..index+1]];
+            splitOnLetter(s, index+1, results+[s[index..index+1]])
+        else results
+    }
+
     function splitHelper(s: string, separator: string, index: nat, sindex: nat, results: seq<string>): seq<seq<char>>
         requires index <= |s|
         requires sindex <= |s|
         requires sindex <= index
-        // requires forall ss: string :: ss in results ==> NotContains(ss,separator)
-        // ensures forall ss :: ss in splitHelper(s, separator, index, sindex, results) ==> NotContains(ss, separator)
+        requires |separator| > 0
+        requires |results| <= index
+        requires |results| == 0 ==> sindex == 0
+        requires |results| > 0 ==> nextStartingIndex(sindex, separator, results)
+        requires partialSumSeq(results, separator) == s[..sindex]
+        ensures results <= splitHelper(s, separator, index, sindex, results)
+        ensures 1 <= |splitHelper(s, separator, index, sindex, results)| <= |s|+1
+        ensures (|splitHelper(s,separator, index, sindex, results)|-1)*|separator| + sumLength(splitHelper(s,separator, index, sindex, results)) == |s|
+        ensures sumSeq(splitHelper(s, separator, index, sindex, results), separator) == s
         decreases |s| - index
     {
-        if index >= |s| then results + [s[sindex..index]]
-        else if |separator| == 0 && index == |s|-1 then splitHelper(s, separator, index+1, index, results)
-        else if |separator| == 0 then 
-        assert separator == [];
-        assert s[sindex..index+1] != [];
-        splitHelper(s, separator, index+1, index+1, results + [s[sindex..(index+1)]])
-        else if index+|separator| > |s| then splitHelper(s, separator, |s|, sindex, results)
-        else if s[index..index+|separator|] == separator then splitHelper(s, separator, index+|separator|, index+|separator|, results + [s[sindex..index]])
+        if index == |s| then
+            var next := results+ [s[sindex..index]];
+            assert |results| > 0 ==> |results|*|separator| + sumLength(results) == sindex;
+            sumSeqPartial(next, separator);
+            assert results == next[..|next|-1];
+            assert partialSumSeq(next[..|next|-1], separator) == s[..sindex];
+            next
+        else if index+|separator| > |s| then
+            splitHelper(s, separator, |s|, sindex, results)
+        else if s[index..index+|separator|] == separator then
+            partialSumSeqConcat(results,[s[sindex..index]], separator);
+            splitHelper(s, separator, index+|separator|, index+|separator|, results + [s[sindex..index]])
         else splitHelper(s, separator, index+1, sindex, results)
     }
 
-    function split(s: string, separator: string): seq<string> 
-        ensures split(s, separator) == splitHelper(s, separator, 0,0, [])
+    lemma {:induction } SplitOnLettersSlice(s: string, i: int)
+        requires 0 <= i < |s|
+        ensures sumSeq(splitOnLetter(s, 0, [])[i..], "") == s[i..]
+        decreases |s|-i
     {
-        splitHelper(s, separator, 0, 0, [])
+    }
+
+    lemma SplitOnLettersIdemp(s: string)
+        ensures sumSeq(splitOnLetter(s, 0, []), "") == s
+    {
+        if |s| == 0 {
+            assert s == "";
+            assert splitOnLetter(s, 0,[]) ==[];
+            assert sumSeq([],"") == "";
+            assert sumSeq(splitOnLetter(s, 0, []), "") == s;
+        }else if |s| == 1 {
+            assert splitOnLetter(s, 0,[]) ==[s[0..1]];
+        }else{
+            assert s == s[0..];
+            SplitOnLettersSlice(s, 0);
+            assert |splitOnLetter(s,0,[])| == |s|;
+            assert 0 <= 1 < |splitOnLetter(s, 0, [])|;
+            assert splitOnLetter(s, 0, [])[0] == s[0..1];
+        }
+    }
+
+    function split(s: string, separator: string): seq<string> 
+        ensures sumSeq(split(s, separator), separator) == s
+    {
+        if |separator| == 0 then
+            SplitOnLettersIdemp(s);
+            splitOnLetter(s, 0, [])
+        else
+            splitHelper(s, separator, 0, 0, [])
     }
 
     predicate Contains(haystack: string, needle: string)
-        // ensures !NotContainsThree(haystack, needle)
         ensures Contains(haystack, needle) <==> exists k :: 0 <= k <= |haystack| && needle <= haystack[k..] 
         ensures Contains(haystack, needle) <==> exists i :: 0 <= i <= |haystack| && (needle <= haystack[i..])
         ensures !Contains(haystack, needle) <==> forall i :: 0 <= i <= |haystack| ==> !(needle <= haystack[i..])
@@ -47,4 +174,6 @@ module Split {
     function splitOnDoubleBreak(s: string): seq<string> {
         if Contains(s, "\r\n") then split(s,"\r\n\r\n") else split(s,"\n\n")
     }
+
+    export provides split, Contains, splitOnBreak, splitOnDoubleBreak, sumSeq
 }
